policies/PVI.v
@@ -128,6 +128,8 @@ Module PVI <: Policy.
   Definition RetT       := Passthrough.RetT policy_state val_tag control_tag.
   Definition AccessT    := Passthrough.AccessT policy_state val_tag control_tag.
   Definition AssignT    := Passthrough.AssignT policy_state val_tag control_tag.
+  Definition CoalesceT  := Passthrough.CoalesceT policy_state val_tag vt_eq_dec.
+  Definition EffectiveT := Passthrough.EffectiveT val_tag def_tag. 
   Definition UnopT      := Passthrough.UnopT policy_state val_tag control_tag.
   Definition SplitT     := Passthrough.SplitT policy_state val_tag control_tag.
   Definition LabelT     := Passthrough.LabelT policy_state control_tag.
